Fix CRC-32 table generation.

code/c/Yazi_CRC32_Table_Codegen.c
@@ -1,6 +1,6 @@
 #include <stdio.h>
 #include <stdint.h>
-#include "Yazi_CRC32_Table.h"
+#include "Yazi_CRC32_Impl.h"
 
 int main(int argc, const char **argv) {
   uint32_t table[4][256];
@@ -9,7 +9,12 @@ int main(int argc, const char **argv) {
   uint32_t matrix[32];
   gen_matrix_table(matrix);
 
-  printf("static uint32_t crc32_table[4][256] = {\n");
+  printf(
+    "#ifndef __GNUC__\n"
+    "#include <string.h>\n"
+    "#endif\n"
+    "#include \"Yazi_CRC32_Impl.h\"\n\n"
+    "static uint32_t crc32_table[4][256] = {\n");
   
   for (int i = 0; i < 4; i++) {
     if (i == 0) {
@@ -31,48 +36,25 @@ int main(int argc, const char **argv) {
 
   printf(
     "\n};\n\n"
-    "uint32_t crc32_combine64(uint32_t crc1, uint32_t crc2, uint64_t len2) {\n"
-    "  uint32_t m0[32];\n"
-    "  uint32_t m1[32] = {\n");
+    "static uint32_t magic_matrix[32] = {");
 
   for (int i = 0; i < 32; i++) {
-    printf("0x%.8xUL, ", matrix[i]);
-    if (i > 0 && i % 5 == 0) {
+    if (i % 5 == 0) {
       printf("\n  ");
     }
+    printf("0x%.8xUL, ", matrix[i]);
   }
+
+  printf(
+    "\n};\n\n"
+    "static inline void init_magic_matrix(uint32_t *m) {\n");
   
   printf(
-    "  \n};\n"
-    "  if (len2 == 0) {\n"
-    "    return crc1;\n"
-    "  }\n\n"
-    "  for (;;) {\n"
-    "    if (len2 & 1) {\n"
-    "      crc1 = Yazi_CRC32_Impl_gf2_matrix_times((uint32_t *)m1, crc1);\n"
-    "    }\n\n"
-    "    len2 >>= 1;\n"
-    "    if (len2 > 0) {\n"
-    "      Yazi_CRC32_Impl_gf2_matrix_square((uint32_t *)m1, (uint32_t *)m0);\n"
-    "      if (len2 & 1) {\n"
-    "        crc1 = Yazi_CRC32_Impl_gf2_matrix_times((uint32_t *)m0, crc1);\n"
-    "      }\n"
-    "      len2 >>= 1;\n"
-    "      if (len2 > 0) {\n"
-    "        Yazi_CRC32_Impl_gf2_matrix_square((uint32_t *)m0, (uint32_t *)m1);\n"
-    "      } else {\n"
-    "        break;\n"
-    "      }\n"
-    "    } else {\n"
-    "      break;\n"
-    "    }\n"
-    "  }\n\n"
-    "  return crc1 ^ crc2;\n}\n\n"
-    "uint32_t crc32_combine(uint32_t crc1, uint32_t crc2, uint32_t len2) {\n"
-    "  return crc32_combine64(crc1, crc2, len2);\n"
-    "}\n\n"
-    "unsigned int crc32(unsigned int crc, const unsigned char *buf, unsigned int len) {\n"
-    "  return Yazi_CRC32_Impl_crc32_impl((uint32_t *)crc32_table, crc, len, (uint8_t *) buf);\n"
+    "#ifdef __GNUC__\n"
+    "  __builtin_memcpy(m, magic_matrix, sizeof(magic_matrix));\n"
+    "#else\n"
+    "  memcpy(m, magic_matrix, sizeof(magic_matrix);\n"
+    "#endif\n"
     "}\n");
 
   return 0;
