code/Yazi.CRC32.Impl.fsti
@@ -1,6 +1,8 @@
 module Yazi.CRC32.Impl
 
 module B = LowStar.Buffer
+module Cast = FStar.Int.Cast
+module CB = LowStar.ConstBuffer
 module Ghost = FStar.Ghost
 module HS = FStar.HyperStack
 module U32 = FStar.UInt32
@@ -78,8 +80,10 @@ private let crc32_pre_cond
   B.length buf == len' /\ B.length d.base == d.blen /\ Seq.length d.data == d.dlen /\
   Spec.crc32_matched d.dlen d.data crc true
 
-[@ (CPrologue
-  "unsigned int crc32(unsigned int crc, const unsigned char *buf, unsigned int len);")]
+private type matrix_buf = B.lbuffer U32.t 32
+
+[@ (CPrologue "#ifndef YAZI_CRC32_TABLE_GEN")
+   (CEpilogue "#endif")]
 val crc32_impl:
     tg: table_group
   -> crc: U32.t
@@ -95,30 +99,9 @@ val crc32_impl:
     B.(modifies loc_none h0 h1) /\
     Spec.crc32_matched (d.dlen + U32.v len) (Seq.append d.data (B.as_seq h1 buf)) res true)
 
-private type matrix_buf = B.lbuffer U32.t 32
-
-val gf2_matrix_times:
-    nzeros: Ghost.erased pos
-  -> buf: matrix_buf
-  -> vec: U32.t
-  -> ST.Stack (Spec.matrix_times_product nzeros vec)
-  (requires fun h -> Spec.is_matrix_buf h nzeros buf)
-  (ensures fun h0 res h1 -> B.(modifies loc_none h0 h1))
-
-[@ (CPrologue
-  "uint32_t crc32_combine64(uint32_t crc1, uint32_t crc2, uint64_t len2);uint32_t crc32_combine(uint32_t crc1, uint32_t crc2, uint32_t len2);")]
-val gf2_matrix_square:
-    nzeros: Ghost.erased pos
-  -> b0: matrix_buf
-  -> b1: matrix_buf
-  -> ST.Stack unit
-  (requires fun h -> B.live h b1 /\ B.disjoint b0 b1 /\ Spec.is_matrix_buf h nzeros b0)
-  (ensures fun h0 _ h1 ->
-    let open FStar.Mul in
-    B.modifies (B.loc_buffer b1) h0 h1 /\
-    Spec.is_matrix_buf h1 (nzeros * 2) b1)
-
-val crc32_combine_impl:
+[@ (CPrologue "#ifndef YAZI_CRC32_TABLE_GEN")
+   (CEpilogue "#endif")]
+val crc32_combine64:
     s1: Ghost.erased (Seq.seq U8.t)
   -> s2: Ghost.erased (Seq.seq U8.t)
   -> crc1: U32.t
@@ -132,3 +115,48 @@ val crc32_combine_impl:
     (ensures fun h0 res h1 ->
       B.(modifies loc_none h0 h1) /\
       Spec.crc32_matched (Seq.length s1 + Seq.length s2) (Seq.append s1 s2) res true)
+
+[@ (CPrologue "#ifndef YAZI_CRC32_TABLE_GEN")
+   (CEpilogue "#endif")]
+let crc32_combine (s1 s2: Ghost.erased (Seq.seq U8.t)) (crc1 crc2 length: U32.t):
+ST.Stack U32.t
+(requires fun h ->
+  Spec.crc32_matched (Seq.length s1) s1 crc1 true /\
+  Spec.crc32_matched (Seq.length s2) s2 crc2 true /\
+  U32.v length == Seq.length s2)
+(ensures fun h0 res h1 ->
+  B.(modifies loc_none h0 h1) /\
+  Spec.crc32_matched (Seq.length s1 + Seq.length s2) (Seq.append s1 s2) res true) =
+  crc32_combine64 s1 s2 crc1 crc2 (Cast.uint32_to_uint64 length)
+
+[@ (CPrologue "#ifdef YAZI_CRC32_TABLE_GEN")
+   (CEpilogue "#endif")]
+val gen_crc32_table:
+    t8: Spec.table_buf
+  -> t16: Spec.table_buf
+  -> t24: Spec.table_buf
+  -> t32: Spec.table_buf
+  -> ST.Stack unit
+  (requires fun h ->
+    B.live h t8 /\ B.live h t16 /\ B.live h t24 /\ B.live h t32 /\
+    B.disjoint t8 t16 /\ B.disjoint t8 t24 /\ B.disjoint t8 t32 /\
+    B.disjoint t16 t24 /\ B.disjoint t16 t32 /\ B.disjoint t24 t32)
+  (ensures fun h0 _ h1 ->
+    B.modifies 
+      (B.loc_buffer t8 `B.loc_union`
+      B.loc_buffer t16 `B.loc_union`
+      B.loc_buffer t24 `B.loc_union`
+      B.loc_buffer t32)
+      h0 h1 /\
+    Spec.table_correct 8 h1 t8 /\
+    Spec.table_correct 16 h1 t16 /\
+    Spec.table_correct 24 h1 t24 /\
+    Spec.table_correct 32 h1 t32)
+
+[@ (CPrologue "#ifdef YAZI_CRC32_TABLE_GEN")
+   (CEpilogue "#endif")]
+val gen_matrix_table:
+    buf: Spec.matrix_buf
+  -> ST.Stack unit
+  (requires fun h -> B.live h buf)
+  (ensures fun h0 _ h1 -> B.modifies (B.loc_buffer buf) h0 h1 /\ Spec.is_matrix_buf h1 8 buf)
